iris/UTreeAdequacy.v
@@ -134,8 +134,6 @@ Section TreeAdequacy.
     iMod (tree_sup_of_bump c r with "Hturn") as "#Hsup".
     iModIntro.
     iApply (init_boot_of_sup (bv_unsigned InodeInv.ROOTINO) fdt0).
-    - (* the output licence, free at the trivial console claim *)
-      iIntros "_". by iApply (cons_licence_triv Hcons).
     - (* the supply, at the era's record equation *)
       rewrite /AppInv.app_sup Heq.
       cbn [AppCfg.app_pred AppCfg.app_run AppCfg.app_names
